adjust cont stack ghost state

src/imp_plus/lifting2.v
@@ -29,7 +29,7 @@ Ltac expr_det := match goal with H1 : eval_expr' ?a ?b ?v1, H2 : eval_expr' ?a ?
 
 Section wp.
 
-Context `{!gen_heapGS loc val Σ} `{!envGS val Σ} `{!invGS_gen hlc Σ} `{!inG Σ (excl_authR nat)}.
+Context `{!gen_heapGS loc val Σ} `{!envGS val Σ} `{!invGS_gen hlc Σ} `{!inG Σ (excl_authR (leibnizO cont))}.
 
 Variable (F : func_env).
 Variable (γ : gname).
@@ -46,7 +46,7 @@ Definition stack_depth k := snd (cont_to_stack k).
 Canonical Structure imp_plus_lang := Language (implang_mixin F).
 
 Definition state_ctx s := (gen_heap_interp s.2 ∗
-  ∃ ρ0 n, env_auth (<[n := s.1]>ρ0) ∗ own γ (●E n))%I.
+  ∃ k, let '(ρ0, n) := cont_to_stack k in env_auth (<[n := s.1]>ρ0) ∗ own γ (●E (k : leibnizO cont)))%I.
 
 Global Instance implang_irisG : irisGS_gen hlc imp_plus_lang Σ := {
   iris_invGS := _;
@@ -56,10 +56,10 @@ Global Instance implang_irisG : irisGS_gen hlc imp_plus_lang Σ := {
   state_interp_mono _ _ _ _ := fupd_intro _ _;
 }.
 
-Definition stack_top n := (⎡own γ (◯E n)⎤ ∗ stack_level n)%I.
+Definition stack_match k := (⎡own γ (◯E k)⎤ ∗ stack_level (stack_depth k))%I.
 
-Definition wp_sk E s k Q := (stack_top (stack_depth k) -∗
-  ⎡wp NotStuck E (s, k) (λ _, ∃ n', own γ (◯E n') ∗ Q n')⎤)%I.
+Definition wp_sk E s k Q := (stack_match k -∗
+  ⎡wp NotStuck E (s, k) (λ _, ∃ k', own γ (◯E k') ∗ Q (stack_depth k'))⎤)%I.
 
 Record postassert :=
   { Qnormal : assert; Qbreak : assert; Qcontinue : assert; Qreturn : val → assert }.
@@ -104,12 +104,12 @@ Proof.
   iIntros "H %% Hguard"; by iApply "Hguard".
 Qed.
 
-Lemma var_e : forall n x v s,
-  stack_top n ∗ x ↦v v ∗ ⎡state_ctx s⎤ ⊢ ⌜s.1 !! x = Some v⌝.
+Lemma var_e : forall k x v s,
+  stack_match k ∗ x ↦v v ∗ ⎡state_ctx s⎤ ⊢ ⌜s.1 !! x = Some v⌝.
 Proof.
-  intros; rewrite /state_ctx /stack_top /stack_level.
+  intros; rewrite /state_ctx /stack_match /stack_level.
   split => ?; monPred.unseal.
-  iIntros "((N & <-) & Hx & _ & % & % & Hρ & N')".
+  iIntros "((N & <-) & Hx & _ & % & % & %Hm & Hρ & N')".
   iCombine "N N'" gives %->%excl_auth_agree_L.
   iDestruct (var_e with "[$Hx $Hρ]") as %?.
   by rewrite /env_to_environ lookup_insert in H.
@@ -121,23 +121,24 @@ Lemma var_update : forall n x v v' s,
 Proof.
   intros; rewrite /state_ctx /stack_top /stack_level.
   split => ?; monPred.unseal.
-  iIntros "((N & %H) & Hx & $ & % & % & Hρ & N')"; hnf in H; subst.
+  iIntros "((N & %H) & Hx & $ & % & % & % & Hρ & N')"; hnf in H; subst.
   iCombine "N N'" gives %<-%excl_auth_agree_L.
   iMod (var_update with "[$Hx $Hρ]") as "(? & $)".
   rewrite /set_var lookup_insert insert_insert; by iFrame.
 Qed.
 
-Lemma wp_expr_lift E e Q n s : wp_expr E e Q -∗ stack_top n -∗
+Lemma wp_expr_app E e Q n s : wp_expr E e Q -∗ stack_top n -∗
   ⎡state_ctx s⎤ ={E}=∗ ∃ v, ⌜eval_expr e s.1 s.2 v⌝ ∗ stack_top n ∗
   ⎡state_ctx s⎤ ∗ Q v.
 Proof.
   rewrite /state_ctx; wp_expr.unseal.
-  iIntros "H (N & #L) (Hσ & % & % & Hρ & N')".
+  iIntros "H (N & #L) (Hσ & % & % & % & Hρ & N')".
   iMod ("H" with "[$Hσ $Hρ]") as (?) "(He & ($ & $) & HQ)".
   iCombine "N N'" gives %->%excl_auth_agree_L.
   iFrame; iFrame "#".
   iStopProof; split => ?; rewrite /stack_level; monPred.unseal; rewrite monPred_at_intuitionistically.
-  iIntros "(% & H)"; iApply ("H" with "[//]").
+  iIntros "(% & H) !>"; iSplit => //.
+  iApply ("H" with "[//]").
   by rewrite lookup_insert.
 Qed.
 
@@ -152,7 +153,7 @@ Proof.
   iIntros "H %% Hguard".
   rewrite /wp_sk wp_unfold /wp_pre /=.
   iIntros "N" (?????) "S".
-  iMod (wp_expr_lift with "H N S") as (? He) "(N & S & (% & Hx) & Hpost)".
+  iMod (wp_expr_app with "H N S") as (? He) "(N & S & (% & Hx) & Hpost)".
   rewrite embed_fupd; iApply fupd_mask_intro; first set_solver; iIntros "Hclose".
   iDestruct (var_e with "[$N $Hx $S]") as %Hx.
   iSplit.
@@ -172,44 +173,50 @@ Qed.
 Lemma wp_alloc E x Q : (∃ v0, points_to_var x v0) ∗
   ▷ (∀ l, points_to_var x (LocV l) -∗ l ↦ NumV 0 -∗ Qnormal Q) ⊢ wp E (Salloc x) Q.
 Proof.
-  iIntros "H %% Hguard".
-  rewrite wp_sk_unfold /wp_sk_pre; iRight.
-  iIntros (??) "S".
+  iIntros "H %% Hguard N".
+  rewrite wp_unfold /wp_pre /=.
+  iIntros (?????) "S".
   iDestruct "H" as "((% & Hx) & Hpost)".
-  iApply fupd_mask_intro; first set_solver; iIntros "Hclose" (?) "Hstack".
-  iDestruct (var_e with "[$Hx $S $Hstack]") as %?.
-  iExists _, _, _, _; iSplit.
-  { iPureIntro; by constructor. }
-  iNext; simpl.
-  iMod (var_update with "[$Hx $S $Hstack]") as (?) "(? & Hx & S)".
-  iMod (state_interp_alloc with "S") as "($ & ?)".
+  rewrite embed_fupd; iApply fupd_mask_intro; first set_solver; iIntros "Hclose".
+  iDestruct (var_e with "[$Hx $S $N]") as %Hx.
+  iSplit.
+  { iPureIntro. eexists _, (_,_), (_,_), _; split; first done; split; first done; constructor. }
+  iIntros ((?,?)(?,?)? (-> & -> & H)) "?"; inv H; simpl in *; subst.
+  rewrite embed_fupd; iModIntro; iNext; rewrite embed_fupd; iModIntro.
+  iMod (var_update with "[$Hx $S $N]") as "(N & Hx & S)".
+  iDestruct "S" as "(Hσ & % & % & % & Hρ & $)".
+  iMod (state_interp_alloc with "[$Hσ $Hρ]") as "(($ & $) & ?)".
   { apply next_loc_new. }
-  iMod "Hclose"; iModIntro.
-  iApply (stack_match_embed with "[$]").
-  by iApply "Hguard"; iApply ("Hpost" with "[$]").
+  iMod "Hclose"; rewrite embed_fupd; iModIntro.
+  rewrite bi.sep_emp; iSplit => //.
+  iDestruct "Hguard" as "(Hguard & _)".
+  iApply ("Hguard" with "[-N] N").
+  by iApply ("Hpost" with "[$]").
 Qed.
 
 Lemma wp_store E e1 e2 Q : wp_expr E e2 (λ v, wp_expr E e1 (λ v1, ∃ l v0, ⌜v1 = LocV l⌝ ∧
   l ↦ v0 ∗ ▷ (l ↦ v -∗ Qnormal Q))) ⊢ wp E (Sstore e1 e2) Q.
 Proof.
-  iIntros "H %% Hguard".
-  rewrite wp_sk_unfold /wp_sk_pre; iRight.
-  iIntros (??) "S".
-  wp_expr.unseal.
-  iMod ("H" with "S") as (?) "(He2 & S & H)".
-  wp_expr.unseal.
-  iMod ("H" with "S") as (?) "(He1 & S & % & % & -> & Hl & Hpost)".
-  iApply fupd_mask_intro; first set_solver; iIntros "Hclose" (?) "Hstack".
-  iDestruct (state_interp_load with "S Hl") as %?.
-  iDestruct ("He1" with "[Hstack]") as %?; first by iApply stack_env_match.
-  iDestruct ("He2" with "[Hstack]") as %?; first by iApply stack_env_match.
-  iExists _, _, _, _; iSplit.
-  { iPureIntro; by econstructor. }
-  iNext.
-  iMod (state_interp_store with "S Hl") as "($ & ?)"; iFrame.
-  iMod "Hclose"; iModIntro.
-  iApply (stack_match_embed with "[$]").
-  by iApply "Hguard"; iApply "Hpost".
+  iIntros "H %% Hguard N".
+  rewrite wp_unfold /wp_pre /=.
+  iIntros (?????) "S".
+  iMod (wp_expr_app with "H N S") as (? He2) "(N & S & H)".
+  iMod (wp_expr_app with "H N S") as (? He1) "(N & S & % & % & -> & Hl & Hpost)".
+  rewrite embed_fupd; iApply fupd_mask_intro; first set_solver; iIntros "Hclose".
+  iDestruct "S" as "(Hσ & % & % & %Hm & Hρ & ?)".
+  iDestruct (state_interp_load with "[$Hσ $Hρ] Hl") as %Hl.
+  iSplit.
+  { iPureIntro. eexists _, (_,_), (_,_), _; split; first done; split; first done; by econstructor. }
+  iIntros ((?,?)(?,?)? (-> & -> & H)) "?"; inv H; simpl in *; subst.
+  eapply eval_expr_det in He2; last done.
+  eapply eval_expr_det in He1; last done; inv He1.
+  rewrite embed_fupd; iModIntro; iNext; rewrite embed_fupd; iModIntro.
+  iMod (state_interp_store with "[$Hσ $Hρ] Hl") as "(($ & ?) & ?)"; iFrame.
+  iMod "Hclose"; rewrite embed_fupd; iModIntro.
+  rewrite bi.sep_emp; iSplit => //.
+  iDestruct "Hguard" as "(Hguard & _)".
+  iApply ("Hguard" with "[-N] N").
+  by iApply ("Hpost" with "[$]").
 Qed.
 
 Definition set_normal Q R :=
@@ -217,45 +224,49 @@ Definition set_normal Q R :=
 
 Lemma wp_seq E s1 s2 Q : ▷ wp E s1 (set_normal Q (▷ wp E s2 Q)) ⊢ wp E (Sseq s1 s2) Q.
 Proof.
-  iIntros "H %% Hguard".
-  rewrite wp_sk_unfold /wp_sk_pre; iRight.
-  iIntros (??) "S".
-  iApply fupd_mask_intro; first set_solver; iIntros "Hclose" (?) "Hstack".
-  iExists _, _, _, _; iSplit.
-  { iPureIntro; by econstructor. }
-  iNext; iFrame.
-  iMod "Hclose" as "_"; iModIntro.
-  iApply (stack_match_embed with "[$]").
-  iApply "H".
+  iIntros "H %% Hguard N".
+  rewrite wp_unfold /wp_pre /=.
+  iIntros (?????) "S".
+  rewrite embed_fupd; iApply fupd_mask_intro; first set_solver; iIntros "Hclose".
+  iSplit.
+  { iPureIntro. eexists _, (_,_), (_,_), _; split; first done; split; first done; by econstructor. }
+  iIntros ((?,?)(?,?)? (-> & -> & H)) "?"; inv H; simpl in *; subst.
+  rewrite embed_fupd; iModIntro; iNext; rewrite embed_fupd; iModIntro.
+  iFrame; rewrite bi.sep_emp.
+  iMod "Hclose" as "_"; rewrite embed_fupd; iModIntro.
+  iApply ("H" with "[-N] [N]"); last done.
   rewrite /guarded.
   iSplit => /=; last by iDestruct "Hguard" as "[_ $]".
-  iIntros "H"; rewrite (wp_sk_unfold _ _ (Kseq _ _)) /wp_sk_pre; iRight.
-  iIntros (??) "S".
-  iApply fupd_mask_intro; first set_solver; iIntros "Hclose" (?) "Hstack".
-  iExists _, _, _, _; iSplit.
-  { iPureIntro; by econstructor. }
-  iNext; iFrame.
-  iMod "Hclose" as "_"; iModIntro.
-  iApply (stack_match_embed with "[$]").
-  by iApply "H".
+  iIntros "H N"; rewrite wp_unfold /wp_pre /=.
+  iIntros (?????) "S".
+  rewrite embed_fupd; iApply fupd_mask_intro; first set_solver; iIntros "Hclose".
+  iSplit.
+  { iPureIntro. eexists _, (_,_), (_,_), _; split; first done; split; first done; by econstructor. }
+  iIntros ((?,?)(?,?)? (-> & -> & H)) "?"; inv H; simpl in *; subst.
+  inv H5.
+  rewrite embed_fupd; iModIntro; iNext; rewrite embed_fupd; iModIntro.
+  iFrame; rewrite bi.sep_emp.
+  iMod "Hclose" as "_".
+  rewrite embed_fupd; iModIntro.
+  by iApply ("H" with "Hguard").
 Qed.
 
 Lemma wp_if E e s1 s2 Q : wp_expr E e (λ v, ∃ n, ⌜v = NumV n⌝ ∧
   ▷ wp E (if Z.eqb n 0 then s2 else s1) Q) ⊢ wp E (Sif e s1 s2) Q.
 Proof.
-  iIntros "H %% Hguard".
-  rewrite wp_sk_unfold /wp_sk_pre; iRight.
-  iIntros (??) "S".
-  wp_expr.unseal.
-  iMod ("H" with "S") as (?) "(He & S & % & -> & H)".
-  iApply fupd_mask_intro; first set_solver; iIntros "Hclose" (?) "Hstack".
-  iDestruct ("He" with "[Hstack]") as %?; first by iApply stack_env_match.
-  iExists _, _, _, _; iSplit.
-  { iPureIntro; by econstructor. }
-  iNext; iFrame.
-  iMod "Hclose" as "_"; iModIntro.
-  iApply (stack_match_embed with "[$]").
-  by iApply "H".
+  iIntros "H %% Hguard N".
+  rewrite wp_unfold /wp_pre /=.
+  iIntros (?????) "S".
+  iMod (wp_expr_app with "H N S") as (? He) "(N & S & % & -> & H)".
+  rewrite embed_fupd; iApply fupd_mask_intro; first set_solver; iIntros "Hclose".
+  iSplit.
+  { iPureIntro. eexists _, (_,_), (_,_), _; split; first done; split; first done; by econstructor. }
+  iIntros ((?,?)(?,?)? (-> & -> & H)) "?"; inv H; simpl in *; subst.
+  eapply eval_expr_det in He; last done; inv He.
+  rewrite embed_fupd; iModIntro; iNext; rewrite embed_fupd; iModIntro.
+  iMod "Hclose" as "_".
+  iFrame; rewrite bi.sep_emp embed_fupd; iModIntro.
+  by iApply ("H" with "Hguard").
 Qed.
 
 Definition loop_post Q R :=
@@ -265,49 +276,57 @@ Lemma wp_while E e s Q : wp_expr E e (λ v, ∃ n, ⌜v = NumV n⌝ ∧
   ▷ if Z.eqb n 0 then Qnormal Q else wp E s (loop_post Q (▷ wp E (Swhile e s) Q))) ⊢
   wp E (Swhile e s) Q.
 Proof.
-  iIntros "H %% Hguard".
-  rewrite wp_sk_unfold /wp_sk_pre; iRight.
-  iIntros (??) "S".
-  wp_expr.unseal.
-  iMod ("H" with "S") as (?) "(He & S & % & -> & H)".
-  iApply fupd_mask_intro; first set_solver; iIntros "Hclose" (?) "Hstack".
-  iDestruct ("He" with "[Hstack]") as %?; first by iApply stack_env_match.
+  iIntros "H %% Hguard N".
+  rewrite wp_unfold /wp_pre /=.
+  iIntros (?????) "S".
+  iMod (wp_expr_app with "H N S") as (? He) "(N & S & % & -> & H)".
+  rewrite embed_fupd; iApply fupd_mask_intro; first set_solver; iIntros "Hclose".
   destruct (Z.eqb_spec n 0).
-  - subst; iExists _, _, _, _; iSplit.
-    { iPureIntro; by apply WhileFS. }
-    iNext; iFrame.
-    iMod "Hclose" as "_"; iModIntro.
-    iApply (stack_match_embed with "[$]").
-    by iApply "Hguard".
-  - iExists _, _, _, _; iSplit.
-    { iPureIntro; by eapply WhileTS. }
-    iNext; iFrame.
-    iMod "Hclose" as "_"; iModIntro.
-    iApply (stack_match_embed with "[$]").
-    iApply "H".
+  - subst; iSplit.
+    { iPureIntro. eexists _, (_,_), (_,_), _; split; first done; split; first done; by econstructor. }
+    iIntros ((?,?)(?,?)? (-> & -> & H)) "?"; inv H; simpl in *; subst.
+    eapply eval_expr_det in He; last done; inv He.
+    rewrite embed_fupd; iModIntro; iNext; rewrite embed_fupd; iModIntro.
+    iMod "Hclose"; rewrite embed_fupd; iModIntro.
+    iFrame; rewrite bi.sep_emp.
+    iDestruct "Hguard" as "(Hguard & _)".
+    by iApply ("Hguard" with "[-N] N").
+  - iSplit.
+    { iPureIntro. eexists _, (_,_), (_,_), _; split; first done; split; first done; simpl; by eapply WhileTS. }
+    iIntros ((?,?)(?,?)? (-> & -> & H)) "?"; inv H; simpl in *; subst.
+    2: { eapply eval_expr_det in He; last done; inv He. }
+    eapply eval_expr_det in He; last done; inv He.
+    rewrite embed_fupd; iModIntro; iNext; rewrite embed_fupd; iModIntro.
+    iMod "Hclose" as "_"; rewrite embed_fupd; iModIntro.
+    iFrame; rewrite bi.sep_emp.
+    iApply ("H" with "[-N] [N]"); last done.
     rewrite /guarded.
     iSplit; [|iSplit; [|iSplit]]; simpl.
-    + iIntros "H"; rewrite (wp_sk_unfold _ _ (Kwhile _ _ _)) /wp_sk_pre; iRight.
-      iIntros (??) "S".
-      iApply fupd_mask_intro; first set_solver; iIntros "Hclose" (?) "Hstack".
-      iExists _, _, _, _; iSplit.
-      { iPureIntro; by econstructor. }
-      iNext; iFrame.
-      iMod "Hclose" as "_"; iModIntro.
-      iApply (stack_match_embed with "[$]").
-      by iApply "H".
+    + iIntros "H N"; rewrite wp_unfold /wp_pre /=.
+      iIntros (?????) "S".
+      rewrite embed_fupd; iApply fupd_mask_intro; first set_solver; iIntros "Hclose".
+      iSplit.
+      { iPureIntro. eexists _, (_,_), (_,_), _; split; first done; split; first done; simpl; by constructor. }
+      iIntros ((?,?)(?,?)? (-> & -> & H)) "?"; inv H; simpl in *; subst.
+      inv H5.
+      rewrite embed_fupd; iModIntro; iNext; rewrite embed_fupd; iModIntro.
+      iMod "Hclose"; rewrite embed_fupd; iModIntro.
+      iFrame; rewrite bi.sep_emp.
+      by iApply ("H" with "[-N] [N]").
     + iIntros "H"; iExists _, _, _; iSplit => //.
       by iApply "Hguard".
     + iIntros "H"; iExists _; iSplit => //.
-      rewrite (wp_sk_unfold _ _ (Kwhile _ _ _)) /wp_sk_pre; iRight.
-      iIntros (??) "S".
-      iApply fupd_mask_intro; first set_solver; iIntros "Hclose" (?) "Hstack".
-      iExists _, _, _, _; iSplit.
-      { iPureIntro; by econstructor. }
-      iNext; iFrame.
-      iMod "Hclose" as "_"; iModIntro.
-      iApply (stack_match_embed with "[$]").
-      by iApply "H".
+      iIntros "N"; rewrite wp_unfold /wp_pre /=.
+      iIntros (?????) "S".
+      rewrite embed_fupd; iApply fupd_mask_intro; first set_solver; iIntros "Hclose".
+      iSplit.
+      { iPureIntro. eexists _, (_,_), (_,_), _; split; first done; split; first done; simpl; by constructor. }
+      iIntros ((?,?)(?,?)? (-> & -> & H)) "?"; inv H; simpl in *; subst.
+      inv H5.
+      rewrite embed_fupd; iModIntro; iNext; rewrite embed_fupd; iModIntro.
+      iMod "Hclose"; rewrite embed_fupd; iModIntro.
+      iFrame; rewrite bi.sep_emp.
+      by iApply ("H" with "[-N] [N]").
     + iDestruct "Hguard" as "(_ & _ & _ & $)".
 Qed.
 
@@ -335,27 +354,29 @@ Proof.
   by inversion 1.
 Qed.
 
-Lemma stack_match_loop ρ r k e s k' : find_loop k = Some (Kwhile e s k') →
-  stack_match ρ r k ⊢ stack_match ρ r k'.
+Lemma stack_depth_loop k e s k' : find_loop k = Some (Kwhile e s k') →
+  stack_depth k = stack_depth k'.
 Proof.
-  intros. rewrite /stack_match /stack_level.
-  rewrite -(cont_to_stack_loop _ _ _ _ H) //.
+  intros; rewrite /stack_depth; f_equal; by eapply cont_to_stack_loop.
 Qed.
 
 Lemma wp_break E Q : Qbreak Q ⊢ wp E Sbreak Q.
 Proof.
-  iIntros "H %% Hguard".
+  iIntros "H %% Hguard N".
   iDestruct "Hguard" as "(_ & Hguard & _)".
-  iDestruct ("Hguard" with "H") as (????) "H".
-  rewrite (wp_sk_unfold _ Sbreak) /wp_sk_pre; iRight.
-  iIntros (??) "S".
-  iApply fupd_mask_intro; first set_solver; iIntros "Hclose" (?) "Hstack".
-  iExists _, _, _, _; iSplit.
-  { iPureIntro; by econstructor. }
-  iNext; iFrame.
-  iMod "Hclose" as "_"; iModIntro.
-  rewrite stack_match_loop //.
-  by iApply (stack_match_embed with "[$]"). 
+  iDestruct ("Hguard" with "H") as (??? Hk) "H".
+  rewrite wp_unfold /wp_pre /=.
+  iIntros (?????) "S".
+  rewrite embed_fupd; iApply fupd_mask_intro; first set_solver; iIntros "Hclose".
+  iSplit.
+  { iPureIntro. eexists _, (_,_), (_,_), _; split; first done; split; first done; by econstructor. }
+  iIntros ((?,?)(?,?)? (-> & -> & H)) "?"; inv H; simpl in *; subst.
+  rewrite embed_fupd; iModIntro; iNext; rewrite embed_fupd; iModIntro.
+  iFrame; rewrite bi.sep_emp.
+  rewrite H5 in Hk; inv Hk.
+  iMod "Hclose" as "_"; rewrite embed_fupd; iModIntro.
+  erewrite stack_depth_loop by done.
+  iApply ("H" with "N").
 Qed.
 
 Lemma find_loop_while k k' : find_loop k = Some k' → ∃ el sl kl, k' = Kwhile el sl kl.
@@ -371,28 +392,30 @@ Proof.
   by inversion 1.
 Qed.
 
-Lemma stack_match_loop' ρ r k k' : find_loop k = Some k' →
-  stack_match ρ r k ⊢ stack_match ρ r k'.
+Lemma stack_depth_loop' k k' : find_loop k = Some k' →
+  stack_depth k = stack_depth k'.
 Proof.
-  split => n. rewrite /stack_match /stack_level.
-  rewrite -(cont_to_stack_loop' _ _ H) //.
+  intros; rewrite /stack_depth; f_equal; by eapply cont_to_stack_loop'.
 Qed.
 
 Lemma wp_continue E Q : Qcontinue Q ⊢ wp E Scontinue Q.
 Proof.
-  iIntros "H %% Hguard".
+  iIntros "H %% Hguard N".
   iDestruct "Hguard" as "(_ & _ & Hguard & _)".
   iDestruct ("Hguard" with "H") as (? Hk') "H".
   edestruct find_loop_while as (? & ? & ? & ?); first done; subst.
-  rewrite (wp_sk_unfold _ Scontinue) /wp_sk_pre; iRight.
-  iIntros (??) "S".
-  iApply fupd_mask_intro; first set_solver; iIntros "Hclose" (?) "Hstack".
-  iExists _, _, _, _; iSplit.
-  { iPureIntro; by econstructor. }
-  iNext; iFrame.
-  iMod "Hclose" as "_"; iModIntro.
-  rewrite stack_match_loop' //.
-  by iApply (stack_match_embed with "[$]").
+  rewrite wp_unfold /wp_pre /=.
+  iIntros (?????) "S".
+  rewrite embed_fupd; iApply fupd_mask_intro; first set_solver; iIntros "Hclose".
+  iSplit.
+  { iPureIntro. eexists _, (_,_), (_,_), _; split; first done; split; first done; by econstructor. }
+  iIntros ((?,?)(?,?)? (-> & -> & H)) "?"; inv H; simpl in *; subst.
+  rewrite embed_fupd; iModIntro; iNext; rewrite embed_fupd; iModIntro.
+  iFrame; rewrite bi.sep_emp.
+  rewrite H5 in Hk'; inv Hk'.
+  iMod "Hclose" as "_"; rewrite embed_fupd; iModIntro.
+  erewrite stack_depth_loop' by done.
+  iApply ("H" with "N").
 Qed.
 
 Definition get_params f := let 'Func params _ _ := f in params.
@@ -417,16 +440,13 @@ Definition call_assert E f vs x R := (⇑ (stack_retainer f -∗ stackframe f vs
     (∃ vs, ⌜stack_size f = length vs⌝ ∧ stackframe f vs) ∗
     ⇓ ((∃ v, points_to_var x v) ∗ ▷ (points_to_var x v -∗ R))))))%I.
 
-Lemma wp_exprs_app E es Q σ ρ : wp_exprs E es Q -∗ ⎡state_interp σ ρ⎤ ={E}=∗
-  ∃ vs, (∀ r k, env_match ρ r -∗ ⌜eval_exprs' es (Build_state r σ k) vs⌝) ∗ ⎡state_interp σ ρ⎤ ∗ Q vs.
+Lemma wp_exprs_app E es Q n s k : wp_exprs E es Q -∗ stack_top n -∗ ⎡state_ctx s⎤ ={E}=∗
+  ∃ vs, ⌜eval_exprs' es (Build_state s.1 s.2 k) vs⌝ ∗ stack_top n ∗ ⎡state_ctx s⎤ ∗ Q vs.
 Proof.
-  iIntros "Hes S"; iInduction es as [|e es] "IH" forall (Q); simpl.
-  - iFrame. iIntros "!> %% ?"; iPureIntro; constructor.
-  - wp_expr.unseal.
-    iMod ("Hes" with "S") as (?) "(He & S & Hes)".
-    iMod ("IH" with "Hes S") as (?) "(Hes & $ & $)".
-    iIntros "!> %% Henv".
-    iDestruct ("He" with "Henv") as %?; iDestruct ("Hes" $! _ k with "Henv") as %?.
+  iIntros "Hes N S"; iInduction es as [|e es] "IH" forall (Q); simpl.
+  - iFrame. iPureIntro; constructor.
+  - iMod (wp_expr_app with "Hes N S") as (??) "(N & S & Hes)".
+    iMod ("IH" with "Hes N S") as (??) "$".
     iPureIntro; by constructor.
 Qed.
 
@@ -440,22 +460,25 @@ Proof.
     eapply IHk; eauto; lia.
 Qed.
 
-Lemma add_frame σ ρ r k x xs vs : ⎡state_interp σ ρ⎤ ∗ stack_match ρ r k ⊢
-  |==> ∃ ρ', ⎡state_interp σ ρ'⎤ ∗ ⇑ (stack_match ρ' (bind_vars xs vs) (Kcall x r k) ∗
+Lemma add_frame s n xs vs : ⎡state_ctx s⎤ ∗ stack_top n ⊢
+  |==> ⎡state_ctx (bind_vars xs vs, s.2)⎤ ∗ ⇑ (stack_top (S n) ∗
     assert_of (λ n, stack_frag n (/ pos_to_Qp (Pos.of_nat (1 + size (bind_vars xs vs))))%Qp 1%Qp (bind_vars xs vs))).
 Proof.
-  intros; rewrite /stack_match /=.
-  destruct (cont_to_stack k) eqn: Hk.
-  iIntros "(Hρ & #Hl & ->)".
-  iMod (state_interp_alloc_frame _ _ (S n) with "Hρ") as "($ & ?)".
+  intros; rewrite /state_ctx /stack_top /=.
+  iIntros "((Hσ & % & % & % & Hρ & N') & N & #L)".
+  iCombine "N N'" gives %->%excl_auth_agree_L.
+  iMod (state_interp_alloc_frame _ _ (S n) with "[$Hσ $Hρ]") as "(($ & $) & ?)".
   { rewrite lookup_insert_ne //.
-    eapply stack_depth_max; eauto. }
+    apply H; lia. }
+  iMod (own_update_2 with "N' N") as "($ & N)".
+  { apply excl_auth_update. }
   iModIntro.
-  iPoseProof (stack_level_up with "Hl") as "$".
-  iModIntro.
-  iSplit; first done.
+  rewrite -!up1_sep -up1_objective; iFrame.
+  iSplit.
+  { iPureIntro; intros; rewrite lookup_insert_ne; last lia; apply H; lia. }
+  iSplit; first by iApply stack_level_up.
   iStopProof; split => ?; rewrite /stack_level; monPred.unseal; rewrite monPred_at_intuitionistically /=.
-  iIntros "((-> & ->) & $)".
+  iIntros "(<- & $)".
 Qed.
 
 Lemma split_stackframe params locals body vs :
@@ -493,20 +516,31 @@ Proof.
       rewrite length_zip_with_l_eq //.
 Qed.
 
-Lemma remove_frame σ ρ r x r0 k q r' : ⎡state_interp σ ρ⎤ ∗ stack_match ρ r (Kcall x r0 k) ∗ assert_of (λ n, stack_frag n q 1%Qp r') ⊢
-  |==> ∃ ρ', ⎡state_interp σ ρ'⎤ ∗ ⇓ stack_match ρ' r0 k.
+(*Lemma remove_frame s r0 n q r' :
+  ⎡state_ctx s⎤ ∗ stack_top (S n) ∗ assert_of (λ n, stack_frag n q 1%Qp r') ⊢
+  |==> ⎡state_ctx (r0, s.2)⎤ ∗ ⇓ stack_top n.
 Proof.
-  intros; rewrite /stack_match /=.
-  destruct (cont_to_stack k) eqn: Hk.
-  iIntros "(Hρ & (#Hl & ->) & H)".
-  iMod (state_interp_dealloc_frame _ _ (S n) with "[$Hρ H]") as "$".
+  intros; rewrite /state_ctx /stack_top /=.
+  iIntros "((Hσ & % & % & % & Hρ & N') & (N & #Hl) & H)".
+  iCombine "N N'" gives %[=]%excl_auth_agree_L; subst.
+  iMod (state_interp_dealloc_frame _ _ (S n) with "[$Hσ $Hρ H]") as "($ & ?)".
   { iApply (stack_level_embed with "Hl H"). }
+  iMod (own_update_2 with "N' N") as "($ & N)".
+  { apply excl_auth_update. }
   iModIntro.
-  rewrite -!down1_sep.
+  rewrite -!down1_sep -down1_objective; iFrame.
   iPoseProof (stack_level_down with "Hl") as "$".
-  rewrite -down1_objective; iPureIntro.
-  apply (delete_insert _ _ r).
+  iExists 
+  iClear "#"; iStopProof; do 2 f_equiv.
+  apply (delete_insert _ _ s.(ρ)).
   rewrite lookup_insert_ne //; eapply stack_depth_max; eauto.
+Qed.*)
+
+Lemma eval_exprs_det e s v1 : eval_exprs' e s v1 → forall v2, eval_exprs' e s v2 →
+  v1 = v2.
+Proof.
+  induction 1; inversion 1; subst; try congruence.
+  expr_det; f_equiv; auto.
 Qed.
 
 Lemma wp_call E x f es Q : wp_exprs E es (λ vs, ∃ fd, ⌜F !! f = Some fd ∧
@@ -514,41 +548,43 @@ Lemma wp_call E x f es Q : wp_exprs E es (λ vs, ∃ fd, ⌜F !! f = Some fd ∧
   ▷ call_assert E fd (vs ++ repeat (NumV 0) (length (get_locals fd))) x (Qnormal Q)) ⊢
   wp E (Scall x f es) Q.
 Proof.
-  iIntros "H %% Hguard".
-  rewrite wp_sk_unfold /wp_sk_pre; iRight.
-  iIntros (??) "S".
-  iMod (wp_exprs_app with "H S") as (?) "(Hes & S & %fd & (% & %Hlen & %) & H)".
+  iIntros "H %% Hguard N".
+  rewrite wp_unfold /wp_pre /=.
+  iIntros (?????) "S".
+  iMod (wp_exprs_app with "H N S") as (? Hes) "(N & S & %fd & (%Hf & %Hlen & %Hnodup) & H)".
   destruct fd; simpl in *.
-  iApply fupd_mask_intro; first set_solver; iIntros "Hclose" (?) "Hstack".
-  iDestruct ("Hes" with "[Hstack]") as %?; first by iApply stack_env_match.
-  iExists _, _, _, _; iSplit.
-  { iPureIntro; by econstructor. }
-  iNext.
-  iMod (add_frame with "[$S $Hstack]") as (?) "($ & Hstack)".
-  iMod "Hclose" as "_"; iModIntro; simpl.
+  rewrite embed_fupd; iApply fupd_mask_intro; first set_solver; iIntros "Hclose".
+  iSplit.
+  { iPureIntro. eexists _, (_,_), (_,_), _; split; first done; split; first done; by econstructor. }
+  iIntros ((?,?)(?,?)? (-> & -> & H)) "?"; inv H; simpl in *; subst.
+  eapply eval_exprs_det in Hes; last done; subst.
+  rewrite embed_fupd; iModIntro; iNext; rewrite embed_fupd; iModIntro.
+  iMod (add_frame with "[$S $N]") as "($ & N)".
+  iMod "Hclose" as "_".
   iApply up1_obj_elim; iApply up1_mono; last first.
   { rewrite -(up1_down1 (guarded _ _ _ _)) /call_assert.
-    iCombine "Hguard H Hstack" as "H"; rewrite !up1_sep; iApply "H". }
-  iIntros "(Hguard & H & Hstack & Hframe)".
-  iApply (stack_match_embed with "Hstack").
-  assert (length (func_params ++ func_locals) = length (vs ++ repeat (NumV 0) (length func_locals))).
+    iCombine "Hguard H N" as "H"; rewrite !up1_sep; iApply "H". }
+  iIntros "(Hguard & H & N & Hframe)".
+  rewrite bi.sep_emp.
+  assert (length (func_params ++ func_locals) = length (vs ++ repeat (NumV 0) (length func_locals))) as Hlen'.
   { rewrite !app_length repeat_length; f_equal.
     rewrite -Hlen; by eapply Forall2_length. }
   rewrite split_stackframe //; iDestruct "Hframe" as "(Hret & Hframe)".
-  iApply ("H" with "Hret Hframe").
+  rewrite embed_fupd; iModIntro.
+  iApply ("H" with "Hret Hframe [Hguard]").
   do 3 (iSplit; first iIntros "[]").
-  iIntros (?) "He"; simpl.
-  clear dependent σ; rewrite wp_sk_unfold /wp_sk_pre; iRight.
-  iIntros (??) "S".
-  wp_expr.unseal.
-  iMod ("He" with "S") as (?) "(He & S & Hret & (% & % & Hframe) & Hpost)".
-  iApply fupd_mask_intro; first set_solver; iIntros "Hclose" (?) "Hstack".
-  iDestruct ("He" with "[Hstack]") as %?; first by iApply stack_env_match.
-  iExists _,_, _, _; iSplit.
-  { iPureIntro; by econstructor. }
+  iIntros (?) "He N"; simpl.
+  rewrite wp_unfold /wp_pre /=.
+  iIntros (?????) "S".
+  iMod (wp_expr_app with "He N S") as (? He) "(N & S & Hret & (% & %Hlens & Hframe) & Hpost)".
+  rewrite embed_fupd; iApply fupd_mask_intro; first set_solver; iIntros "Hclose".
+  iSplit.
+  { iPureIntro. eexists _, (_,_), (_,_), _; split; first done; split; first done; by econstructor. }
+  iIntros ((?,?)(?,?)? (-> & -> & H)) "?"; inv H; simpl in *; subst.
+  inv H8.
+  rewrite embed_fupd; iModIntro; iNext; rewrite embed_fupd; iModIntro.
   rewrite -down1_sep down1_later.
-  iNext.
-  iMod (remove_frame with "[$S $Hstack Hret Hframe]") as (?) "(S & Hstack)".
+  iMod (remove_frame with "[$S $N Hret Hframe]") as "(S & N)".
   { iCombine "Hret Hframe" as "H"; rewrite -split_stackframe //.
     rewrite app_length //. }
   iDestruct "Hpost" as "(Hx & Hpost)".
@@ -583,7 +619,7 @@ Qed.
 
 Lemma wp_return E e Q : wp_expr E e (Qreturn Q) ⊢ wp E (Sreturn e) Q.
 Proof.
-  iIntros "H %% Hguard".
+  iIntros "H %% Hguard N".
   iDestruct "Hguard" as "(_ & _ & _ & Hguard)".
   iSpecialize ("Hguard" with "H").
   iStopProof.
@@ -598,164 +634,45 @@ Qed.
 
 End wp.
 
-Module Import wp.
-  Ltac unseal := rewrite /wp !wp_sk_unfold /wp_sk_pre /=.
-End wp.
-
 Section adequacy.
-
-(* generalize? *)
-Definition not_stuck F s σ := (s = skip ∧ σ.(k) = Kstop) ∨
-  (∃ s' σ', step F s σ s' σ').
-
-Record adequate F s (σ1 : state) (φ : state → Prop) := {
-  adequate_result σ2 : σ2.(k) = Kstop →
-   step_star F s σ1 skip σ2 → φ σ2;
-  adequate_not_stuck s2 σ2 :
-   step_star F s σ1 s2 σ2 →
-   not_stuck F s2 σ2
-}.
-
-Lemma adequate_alt F s1 σ1 (φ : state → Prop) :
-  adequate F s1 σ1 φ ↔ ∀ s2 σ2,
-    step_star F s1 σ1 s2 σ2 →
-      ((s2 = skip ∧ σ2.(k) = Kstop) → φ σ2) ∧
-      (not_stuck F s2 σ2).
-Proof.
-  split.
-  - intros []; naive_solver.
-  - constructor; naive_solver.
-Qed.
-
-Inductive nsteps (F : func_env) : nat → stmt → state → stmt → state → Prop :=
-  | nsteps_refl s σ :
-     nsteps F 0 s σ s σ
-  | nsteps_l n s1 σ1 s2 σ2 s3 σ3 :
-     step F s1 σ1 s2 σ2 →
-     nsteps F n s2 σ2 s3 σ3 →
-     nsteps F (S n) s1 σ1 s3 σ3.
-Local Hint Constructors nsteps : core.
-
-Lemma step_star_nsteps F s1 σ1 s2 σ2 :
-  step_star F s1 σ1 s2 σ2 ↔ ∃ n, nsteps F n s1 σ1 s2 σ2.
-Proof.
-  split.
-  - induction 1; firstorder eauto.
-  - intros (n & Hsteps).
-    induction Hsteps; eauto using Step0, Step1.
-Qed.
 
 Definition normal_post `{envGS val Σ} Q :=
   {| Qnormal := Q; Qbreak := False%I; Qcontinue := False%I; Qreturn := λ _, False%I |}.
 
-Section lemmas.
-
-Context `{!gen_heapGS loc val Σ} `{!envGS val Σ} `{!invGS_gen hlc Σ}.
-
-Lemma guarded_stop F Q : ⊢ guarded F ⊤ (normal_post Q) Kstop Q.
+Lemma guarded_stop `{!gen_heapGS loc val Σ} `{!envGS val Σ} `{!invGS_gen hlc Σ} `{!inG Σ (excl_authR nat)}
+  F γ Q : ⊢ guarded F γ ⊤ (normal_post Q) Kstop Q.
 Proof.
   iSplit; last repeat (iSplit; [iIntros "[]"|]); simpl.
-  - iIntros "?"; wp.unseal; iLeft.
-    iSplit => //.
-  - iIntros (?) "He".
-    wp.unseal.
-    wp_expr.unseal.
-    iRight.
-    iIntros (??) "S"; iMod ("He" with "S") as (?) "(_ & _ & [])".
+  - iIntros "? ?"; rewrite wp_unfold /wp_pre /=.
+    rewrite embed_fupd; iModIntro; iExists _; by iApply (stack_top_embed with "[$]").
+  - iIntros (?) "He N".
+    rewrite wp_unfold /wp_pre /=.
+    iIntros (?????) "S".
+    iMod (wp_expr_app with "He N S") as (? He) "(N & S & [])".
 Qed.
 
-Local Lemma wp_not_stuck F s k σ ρ r Q :
-  ⎡state_interp σ ρ⎤ -∗ stack_match ρ r k -∗ wp_sk F ⊤ s k Q ={⊤, ∅}=∗ ⌜not_stuck F s (Build_state r σ k)⌝.
+Lemma wp_adequacy hlc Σ `{!gen_heapGpreS loc val Σ} `{!inG Σ (@envR val)} `{!invGpreS Σ} `{!inG Σ (excl_authR nat)} F (s : stmt) σ φ :
+  (∀ `{!gen_heapGS loc val Σ} `{!envGS val Σ} `{Hinv : !invGS_gen hlc Σ} γ,
+     ⊢ |={⊤}=> wp F γ ⊤ s (normal_post ⌜φ⌝)) →
+  adequate(Λ := imp_plus_lang F) NotStuck (s, Kstop) (∅, σ) (λ _ _, φ).
 Proof.
-  wp.unseal. rewrite /not_stuck.
-  iIntros "Hσ Hr [(% & _) | H]".
-  - iApply fupd_mask_intro; auto.
-  - iMod ("H" with "Hσ") as "H".
-    iDestruct ("H" with "Hr") as (?????) "_"; eauto.
-Qed.
-
-End lemmas.
-
-Lemma eval_expr_det e r m v1 : eval_expr e r m v1 → forall v2, eval_expr e r m v2 →
-  v1 = v2.
-Proof.
-  induction 1; inversion 1; subst; try congruence.
-  - specialize (IHeval_expr1 _ ltac:(eassumption)).
-    specialize (IHeval_expr2 _ ltac:(eassumption)); congruence.
-  - specialize (IHeval_expr _ ltac:(eassumption)); congruence.
-Qed.
-
-Ltac expr_det := match goal with H1 : eval_expr' ?a ?b ?v1, H2 : eval_expr' ?a ?b ?v2 |- _ =>
-  let H := fresh "Heq" in pose proof (eval_expr_det _ _ _ _ H1 _ H2) as H; clear H2; inv H end.
-
-Lemma eval_exprs_det e σ v1 : eval_exprs' e σ v1 → forall v2, eval_exprs' e σ v2 →
-  v1 = v2.
-Proof.
-  induction 1; inversion 1; subst; try congruence.
-  expr_det; f_equiv; auto.
-Qed.
-
-Lemma step_det F s σ s1 σ1 s2 σ2 : step F s σ s1 σ1 → step F s σ s2 σ2 →
-  s1 = s2 ∧ σ1 = σ2.
-Proof.
-  inversion 1; subst; inversion 1; subst; repeat expr_det; try done; try congruence.
-  - by rewrite H0 in H2; inv H2.
-  - by rewrite H0 in H2; inv H2.
-  - by rewrite H0 in H2; inv H2.
-  - by rewrite H0 in H2; inv H2.
-  - rewrite H0 in H8; inv H8. eapply eval_exprs_det in H2; last done. by subst.
-  - by rewrite H1 in H6; inv H6.
-Qed.
-
-Lemma wp_adequacy Σ `{!gen_heapGpreS loc val Σ} `{!inG Σ (@envR val)} `{!invGpreS Σ} F s σ φ :
-  (∀ `{!gen_heapGS loc val Σ} `{!envGS val Σ} `{Hinv : !invGS_gen hlc Σ},
-     ⊢ |={⊤}=> wp F ⊤ s (normal_post ⌜φ⌝)) →
-  adequate F s (Build_state ∅ σ Kstop) (λ _, φ).
-Proof.
-  intros Hwp. apply adequate_alt; intros s2 σ2 H.
-  eapply uPred.pure_soundness.
-  apply step_star_nsteps in H as (n & H).
-  eapply (step_fupdN_soundness_gen _ hlc n n).
-  iIntros (Hinv) "_".
+  intros; eapply wp_adequacy_gen; first done.
+  intros; iIntros.
   iMod (gen_heap_init σ) as (?) "[Hh _]".
   iMod (env_init ∅) as (?) "(He & _)".
-  iPoseProof (monPred_in_entails _ _ (Hwp _ _ _) O with "[]") as "Hwp"; clear Hwp.
-  { by monPred.unseal. }
-  rewrite monPred_at_fupd; iMod "Hwp".
-  rewrite /wp.
-  set (Q := normal_post _); monPred.unseal; subst Q.
-  iSpecialize ("Hwp" with "[//] []").
-  { iApply (monPred_in_entails _ _ (guarded_stop _ _) with "[]"); by monPred.unseal. }
-  iAssert (stack_match {[0 := ∅]} ∅ Kstop O) as "-#Hstack".
-  { rewrite /stack_match /stack_level; by monPred.unseal. }
-
-  set (r := ∅) in *; clearbody r.
-  set (k := Kstop) at 1 2; fold k in H; clearbody k.
-  set (ρ := {[0 := r]}); change {[0 := r]} with ρ; clearbody ρ.
-  set (l := 0); clearbody l.
-  iInduction n as [|n] "IH" forall (σ ρ r k l s H).
-  - inv H.
-    wp.unseal. monPred.unseal.
-    iDestruct "Hwp" as "[Hwp | Hwp]".
-    + iDestruct "Hwp" as "((-> & ->) & >%)".
-      iApply fupd_mask_intro; first set_solver.
-      iIntros "_"; iPureIntro; rewrite /not_stuck /=; auto.
-    + iMod ("Hwp" with "[//] [$Hh $He]") as "Hwp".
-      iDestruct ("Hwp" with "[//] Hstack") as (???? Hstep) "H".
-      iPureIntro; split.
-      * intros (-> & ->); inv Hstep.
-      * right; eauto.
-  - inv H.
-    wp.unseal. monPred.unseal. iDestruct "Hwp" as "[Hwp | Hwp]".
-    { iDestruct "Hwp" as "((-> & ->) & _)"; inv H3. }
-    iMod ("Hwp" with "[//] [$Hh $He]") as "Hwp".
-    iDestruct ("Hwp" with "[//] Hstack") as (???? Hstep) "H".
-    eapply step_det in H3; last done.
-    destruct H3 as (<- & <-).
-    iModIntro; simpl.
-    iModIntro; iNext.
-    iMod "H" as (?) "((Hh & He) & Hstack & H)".
-    iApply ("IH" with "[//] Hh He H Hstack").
+  iMod (own_alloc) as (?) "H"; first apply (excl_auth_valid O); iDestruct "H" as "(? & N)".
+  iExists (λ σ _, state_ctx γ σ), (λ _, True%I).
+  rewrite /state_ctx /=; iFrame.
+  iPoseProof (monPred_in_entails _ _ (H _ _ _ _) O with "[]") as "Hwp"; clear H;
+    monPred.unseal; first done.
+  iMod "Hwp" as "Hwp".
+  rewrite /wp /wp_sk /stack_top /stack_level; monPred.unseal.
+  iSpecialize ("Hwp" with "[//] [] [//] [N]").
+  { iApply (monPred_in_entails with "[-]"); first apply guarded_stop.
+    by monPred.unseal. }
+  { by iFrame. }
+  iApply (wp_wand with "Hwp").
+  iIntros "!> % (% & _ & $)".
 Qed.
 
 End adequacy.
